Prove Trim.trim_ordered

Bdd/Trim.lean
@@ -2,11 +2,11 @@ import Bdd.Basic
 
 namespace Trim
 
-private def trim_pointer [NeZero k] : Pointer m → Pointer k
+private def trim_pointer : Pointer m → Pointer (k + 1)
   | .terminal b => .terminal b
-  | .node j => .node ⟨j.1 % k, Nat.mod_lt j.1 (by rename_i h; rcases h; omega)⟩
+  | .node j => .node ⟨j.1 % (k + 1), Nat.mod_lt j.1 (Nat.zero_lt_succ k)⟩
 
-private def trim_node [NeZero k] : Node n m → Node n k
+private def trim_node : Node n m → Node n (k + 1)
   | ⟨v, l, h⟩ => ⟨v, trim_pointer l, trim_pointer h⟩
 
 def trim (B : Bdd n m) (h1 : k ≤ m) (h2 : ∀ j : Fin m, Pointer.Reachable B.heap B.root (.node j) → j < k) :
@@ -19,6 +19,195 @@ def trim (B : Bdd n m) (h1 : k ≤ m) (h2 : ∀ j : Fin m, Pointer.Reachable B.h
   | .succ l =>
     ⟨Vector.cast (min_eq_left h1) (Vector.map trim_node (B.heap.take (l + 1))), trim_pointer B.root⟩
 
+private def untrim_pointer (h : k ≤ m) : Pointer k → Pointer m
+  | .terminal b => .terminal b
+  | .node j => .node ⟨j.1, Fin.val_lt_of_le _ h⟩
+
+private def untrim_node (h1 : k ≤ m) : Node n k → Node n m
+  | ⟨v, l, h⟩ => ⟨v, untrim_pointer h1 l, untrim_pointer h1 h⟩
+
+private def untrim (B : Bdd (n + 1) k) (h1 : k ≤ m) : Bdd (n + 1) m :=
+  ⟨ Vector.map
+      (untrim_node h1)
+      (Vector.cast
+        (by omega)
+        (B.heap ++ (Vector.replicate (m - k) (⟨0, .terminal false, .terminal false⟩ : Node (n + 1) k)))),
+    untrim_pointer h1 B.root
+  ⟩
+
+private lemma trim_induction {B : Bdd n m} {h1 : k ≤ m} {h2} {motive : ∀ k, Bdd n k → Prop}
+    (base : ∀ b, B.root = .terminal b → motive 0 ⟨(Vector.emptyWithCapacity 0), .terminal b⟩)
+    (step : ∀ l (hl : l + 1 ≤ m), (∀ j : Fin m, Pointer.Reachable B.heap B.root (.node j) → j < l + 1) → motive (l + 1) ⟨Vector.cast (min_eq_left hl) (Vector.map trim_node (B.heap.take (l + 1))), trim_pointer B.root⟩) :
+    motive k (trim B h1 h2) := by
+  unfold trim
+  split
+  next h1 h2 =>
+    split
+    next b heq => exact base b heq
+    next j heq => rw [heq] at h2; have := h2 j .refl; contradiction
+  next l h1 h2 => exact step l h1 h2
+
+private lemma aux {n m} {B : Bdd n m} {l} {j} (h1 : l + 1 ≤ m) (h2 : j < l + 1) :
+    ((Vector.map Trim.trim_node B.heap).extract 0 (l + 1))[j] =
+    (Vector.map (Trim.trim_node (k := l)) B.heap)[j] := by
+  rw [Vector.getElem_extract]
+  simp
+
+private lemma aux' {B : Bdd n m} {l} {j} (h1 : l + 1 ≤ m) (h2 : j < l + 1) :
+    ((Vector.map Trim.trim_node B.heap).extract 0 (l + 1))[j].low =
+    (Vector.map (Trim.trim_node (k := l)) B.heap)[j].low := by
+  congr 1
+  exact aux h1 h2
+
+private lemma untrim_point_trim_point (p : Pointer m) (_ : l + 1 ≤ m) (hp : ∀ j, p = .node j → j < l + 1) : (untrim_pointer (k := l + 1) h (trim_pointer p)) = p := by
+  simp only [trim_pointer]
+  split
+  next => simp [untrim_pointer]
+  next j =>
+    simp only [untrim_pointer]
+    congr
+    simp only [Nat.mod_succ_eq_iff_lt, Nat.succ_eq_add_one]
+    apply hp
+    rfl
+
+private lemma untrim_point_trim_root : (untrim_pointer h1 (trim B h1 h2).root) = B.root := by
+  simp only [trim]
+  split
+  next k h1 h2 =>
+    split
+    next => simp_all [untrim_pointer]
+    next j hj => rw [hj] at h2; have := h2 j .refl; contradiction
+  next l h1 h2 =>
+    simp only [Nat.succ_eq_add_one]
+    apply untrim_point_trim_point
+    · simp_all
+    · intro j hj
+      apply h2
+      rw [← hj]
+      left
+
+private lemma untrim_point_trim_heap_low {B : Bdd n m} {j : Fin k} {h1 : k ≤ m} {hj : Pointer.Reachable B.heap B.root (Pointer.node ⟨j.1, by omega⟩)} {h2} :
+    (untrim_pointer h1 (trim B h1 h2).heap[j.1].low) = (B.heap[j.1]'(by omega)).low := by
+  have := trim_induction (h2 := h2) (h1 := h1) (motive := fun k' B' ↦ ∀ (h1' : k' ≤ m) (j' : Fin k'), Pointer.Reachable B.heap B.root (.node ⟨j', by omega⟩) → Trim.untrim_pointer h1' B'.heap[j'].low = B.heap[j'].low)
+  apply this
+  · intro _ _ _ ⟨_, _⟩; contradiction
+  · intro l hl hl2 h1' j' hj'
+    simp only [Fin.getElem_fin, Vector.getElem_cast]
+    simp only [Vector.take_eq_extract, Vector.map_extract]
+    have := aux h1' (j := j') (B := B) (by omega)
+    calc _
+      _ = Trim.untrim_pointer h1' ((Vector.map Trim.trim_node B.heap))[j'.1].low := by
+        congr 1
+        congr 1
+      _ = B.heap[j'.1].low := by
+        simp only [Vector.getElem_map]
+        simp [trim_node]
+        rw [untrim_point_trim_point (h := hl)]
+        rfl
+        · exact hl
+        · intro j'' hj''
+          apply hl2
+          right
+          · exact hj'
+          · left
+            exact hj''
+  · exact hj
+
+private lemma untrim_point_trim_heap_high {B : Bdd n m} {j : Fin k} {h1 : k ≤ m} {hj : Pointer.Reachable B.heap B.root (Pointer.node ⟨j.1, by omega⟩)} {h2} :
+    (untrim_pointer h1 (trim B h1 h2).heap[j.1].high) = (B.heap[j.1]'(by omega)).high := by
+  have := trim_induction (h2 := h2) (h1 := h1) (motive := fun k' B' ↦ ∀ (h1' : k' ≤ m) (j' : Fin k'), Pointer.Reachable B.heap B.root (.node ⟨j', by omega⟩) → Trim.untrim_pointer h1' B'.heap[j'].high = B.heap[j'].high)
+  apply this
+  · intro _ _ _ ⟨_, _⟩; contradiction
+  · intro l hl hl2 h1' j' hj'
+    simp only [Fin.getElem_fin, Vector.getElem_cast]
+    simp only [Vector.take_eq_extract, Vector.map_extract]
+    have := aux h1' (j := j') (B := B) (by omega)
+    calc _
+      _ = Trim.untrim_pointer h1' ((Vector.map Trim.trim_node B.heap))[j'.1].high := by
+        congr 1
+        congr 1
+      _ = B.heap[j'.1].high := by
+        simp only [Vector.getElem_map]
+        simp [trim_node]
+        rw [untrim_point_trim_point (h := hl)]
+        rfl
+        · exact hl
+        · intro j'' hj''
+          apply hl2
+          right
+          · exact hj'
+          · right
+            exact hj''
+  · exact hj
+
+private lemma trim_reachable_and_edge
+    (hb : Pointer.Reachable (trim B h1 h2).heap (trim B h1 h2).root b) :
+    Pointer.Reachable B.heap B.root (untrim_pointer h1 b) ∧
+    (∀ c, Edge (trim B h1 h2).heap b c → Edge B.heap (untrim_pointer h1 b) (untrim_pointer h1 c)) := by
+  induction hb with
+  | refl =>
+    have hr : Pointer.Reachable B.heap B.root (Trim.untrim_pointer h1 (trim B h1 h2).root) := by
+      rw [untrim_point_trim_root]; left
+    constructor
+    · exact hr
+    · intro c e
+      simp [untrim_point_trim_root]
+      simp [untrim_point_trim_root] at hr
+      cases hh : (trim B h1 h2).root with
+      | terminal t =>
+        rw [hh] at e
+        contradiction
+      | node j' =>
+        rw [hh] at e
+        have : untrim_pointer h1 (Pointer.node j') = B.root := by
+          rw [← hh]
+          simp [untrim_point_trim_root]
+        cases e with
+        | low he =>
+          rw [← this]
+          left
+          rw [← he]
+          simp only [Fin.getElem_fin]
+          symm
+          apply untrim_point_trim_heap_low
+          rw [← this]
+          left
+        | high he =>
+          rw [← this]
+          right
+          rw [← he]
+          simp only [Fin.getElem_fin]
+          symm
+          apply untrim_point_trim_heap_high
+          rw [← this]
+          left
+  | tail r e ih =>
+    rename_i b c
+    constructor
+    · right
+      · exact ih.1
+      · exact ih.2 _ e
+    · intro d hd
+      cases hd with
+      | low hd =>
+        left
+        rw [← hd]
+        simp only [Fin.getElem_fin]
+        symm
+        apply untrim_point_trim_heap_low
+        right
+        · exact ih.1
+        · exact ih.2 _ e
+      | high hd =>
+        right
+        rw [← hd]
+        simp only [Fin.getElem_fin]
+        symm
+        apply untrim_point_trim_heap_high
+        right
+        · exact ih.1
+        · exact ih.2 _ e
+
 lemma trim_ordered {B : Bdd n m} (o : B.Ordered) {h1 : k ≤ m} {h2} : (trim B h1 h2).Ordered := by
   simp only [trim]
   split
@@ -26,7 +215,40 @@ lemma trim_ordered {B : Bdd n m} (o : B.Ordered) {h1 : k ≤ m} {h2} : (trim B h
     split
     next => exact Bdd.Ordered_of_terminal
     next j hj => rw [hj] at h2; have := h2 j .refl; contradiction
-  next _ _ _ l h1 h2 => sorry
+  next _ _ _ l h1 h2 =>
+    intro ⟨x, hx⟩ ⟨y, hy⟩ hxy
+    simp only [Bdd.RelevantMayPrecede, Pointer.MayPrecede, Nat.succ_eq_add_one]
+    have := @o (⟨untrim_pointer (by simp_all) x, (trim_reachable_and_edge (h2 := h2) hx).1⟩ : B.RelevantPointer)
+               (⟨untrim_pointer (by simp_all) y, (trim_reachable_and_edge (h2 := h2) hy).1⟩ : B.RelevantPointer)
+               ((trim_reachable_and_edge (h1 := h1) (h2 := h2) hx).2 y hxy)
+    simp only [Bdd.RelevantMayPrecede, Pointer.MayPrecede, Nat.succ_eq_add_one] at this
+    convert this using 1
+    · cases heq : x with
+      | terminal => simp [Trim.untrim_pointer]
+      | node j =>
+        have := trim_reachable_and_edge (h1 := h1) (h2 := h2) hx
+        rw [heq] at this
+        simp only [Vector.take_eq_extract, Vector.map_extract, Nat.succ_eq_add_one,
+          Pointer.toVar_node_eq, Fin.getElem_fin, Vector.getElem_cast, Fin.coe_eq_castSucc,
+          untrim_pointer, Fin.castSucc_inj]
+        calc _
+          _ = (Vector.map (Trim.trim_node (k := l)) B.heap)[j.1].var := by
+            congr 1
+            apply aux <;> omega
+          _ = (Trim.trim_node (k := l + 1) B.heap[j.1]).var := by simp; rfl
+    · cases heq : y with
+      | terminal => simp [Trim.untrim_pointer]
+      | node j =>
+        have := trim_reachable_and_edge (h1 := h1) (h2 := h2) hy
+        rw [heq] at this
+        simp only [Vector.take_eq_extract, Vector.map_extract, Nat.succ_eq_add_one,
+          Pointer.toVar_node_eq, Fin.getElem_fin, Vector.getElem_cast, Fin.coe_eq_castSucc,
+          untrim_pointer, Fin.castSucc_inj]
+        calc _
+          _ = (Vector.map (Trim.trim_node (k := l)) B.heap)[j.1].var := by
+            congr 1
+            exact aux (B := B) (j := j.1) (l := l) h1 (h2 ⟨j.1, by omega⟩ this.1)
+          _ = (Trim.trim_node (k := l + 1) B.heap[j.1]).var := by simp; rfl
 
 def otrim (O : OBdd n m) (h1 : k ≤ m) (h2 : ∀ j : Fin m, Pointer.Reachable O.1.heap O.1.root (.node j) → j < k) :
     OBdd n k := ⟨trim O.1 h1 h2, trim_ordered O.2⟩
